## 19.
$$
I=\int_{\frac{2}{\sqrt{ 3 }}}^{2} t \sec t\hspace{1mm} dt
$$
Tome:
$$
u=\sec^{-1}t \implies du= \frac{dx}{|x| \sqrt{ x^2 -1 }},\quad dv=t\hspace{1mm}dt \implies v=\frac{t^2}{2}
$$
Assim:
$$
I = \left[ \frac{t^2\sec^{-1}t}{2} \right]_{\frac{2}{\sqrt{ 3 }}}^{2}  - \frac{1}{2}\int_{\frac{2}{\sqrt{ 3 }}}^{2}  \frac{x^2\hspace{1mm}dx}{|x|\sqrt{ x^2 -1}}
$$
Resolvendo a integral*
$$
\int_{\frac{2}{\sqrt{ 3 }}}^{2}  \frac{x^2}{|x|\sqrt{ x^2-1 }}dx = \int_{\frac{2}{\sqrt{ 3 }}}^{2}  \frac{|x|}{\sqrt{ x^2 -1}} \hspace{1mm}\left( t>\frac{2}{\sqrt{ 3 }} \right) = \int_{\frac{2}{\sqrt{ 3 }}}^{2}  \frac{x}{\sqrt{ x^2-1 }} = [\sqrt{ x^2-1 }]_{\frac{2}{\sqrt{ 3 }}}^{2}
$$
$$
I= \left[ \frac{t^2\sec^{-1}t}{2} \right]_{\frac{2}{\sqrt{ 3 }}}^{2} -\frac{1}{2} \left[ \sqrt{ x^2-1 } \right]_{\frac{2}{\sqrt{ 3 }}}^{2}= \left[ \frac{t^2\sec^{-1}t}{2} -\frac{\sqrt{ x^2 -1}}{2} \right]_{\frac{2}{\sqrt{ 3 }}}^{2}
$$
Calculando a definida:
$$
I = \left[ \frac{2^2\sec^{-1}2}{2} -\frac{\sqrt{ \left( 2 \right)^2 -1}}{2} \right] - \left[ \frac{(\frac{2}{\sqrt{ 3 }})^2\sec^{-1}(\frac{2}{\sqrt{ 3 }})}{2} -\frac{\sqrt{ (\frac{2}{\sqrt{ 3 }})^2 -1}}{2} \right]
$$
$$
I = \left[ \frac{2\pi}{3} - \frac{\sqrt{ 3 }}{2}\right] - \left[ \frac{\pi}{9}- \frac{\sqrt{ 3 }}{6}\right] = \frac{5\pi+3\sqrt{ 3 }}{9}
$$
## 23
$$
I= \int e^{2x} \cos 3x\hspace{1mm}dx
$$
Tome:
$$
u=\cos 3x \implies du=-3 \sin 3x\hspace{1mm}dx,\hspace{1mm} dv=e^{2x} \implies v=\frac{e^{2x}}{2} 
$$
$$
I=  \frac{\cos 3x \cdot e^{2x}}{2} - \frac{3}{2} \int e^{2x} \cdot \sin 3x\hspace{1mm}dx
$$
Tome:
$$
u=\sin 3x \implies du=3 \cos 3x \hspace{1mm} dx,\hspace{1mm} dv=e^{2x} \implies v=\frac{e^{2x}}{2} 
$$
$$
I=  \frac{\cos 3x \cdot e^{2x}}{2} - \frac{3}{2} \left[ \sin 3x \cdot \frac{e^{2x}}{2} -\frac{3}{2}\int \cos 3x\cdot e^{2x}dx\right]
$$
$$
I+\frac{9}{4}I=\frac{2 \cos 3x\cdot e^{2x}}{4}- \frac{3\sin 3x\cdot e^{2x}}{4}
$$

$$
I= \frac{e^{2x}}{13}(2\cos 3x-3\sin 3x) + C
$$
## 25
$$
I = \int e^{\sqrt{ 3x+9 }}dx
$$
Tome:
$$
s=\sqrt{ 3x+9  }\implies u^2 = 3x+9 \implies 2u\cdot du = 3\cdot dx \implies dx = \frac{2u\cdot du}{3}
$$
$$
I= \int e^{u}\cdot \frac{2u}{3}\cdot du
$$
$$
x = \frac{2u}{3} \implies dx = \frac{2}{3}du, \hspace{1mm} dv=e^u \implies v=e^u 
$$
Assim:
$$
I= \frac{2u}{3}\cdot e^{u}-\int \frac{2e^{u}}{3}
$$
$$
= \frac{2e^{u}}{3}(u-1)
$$
$$
= \frac{2e^{\sqrt{ 3x+9 }}}{3}(\sqrt{ 3x+9 }-1)+C
$$
## 27
$$
I = \int_{0}^{\pi/3} x\cdot \tan^2x \cdot dx
$$
$$
= \int_{0}^{\pi/3} (x\sec^2x-x)dx = \int_{0}^{\pi/3}x\sec^2x\cdot dx -\int_{0}^{\pi/3} x\cdot dx
$$
Tome:
$$
u = x \implies du = dx, \hspace{1mm} dw= \sec^2 x \implies w = \tan x
$$
$$
I = [x \tan x] - \int \tan x \cdot dx -\int x\cdot dx
$$
**
$$
\int \tan x = \int \frac{\sin x}{\cos x} dx = -\int \frac{1}{u} = -\ln |\cos x|
$$

$$
I = [x \tan x] - [-\ln|\cos x|]-\left[ \frac{x^2}{2} \right]
$$
$$
I = \left[x \tan x +\ln|\cos x| - \frac{x^2}{2} \right]_{0}^{\pi/3}
$$
$$
I = \left[ \frac{\pi\sqrt{ 3 }}{3} + \ln\left( \frac{1}{2}  \right) -\frac{\pi^2}{18}\right] - [0+0-0] = \frac{\pi\sqrt{ 3 }}{3} + \ln\left( \frac{1}{2}  \right) -\frac{\pi^2}{18}
$$

## 29
$$
I = \int \sin(\ln x) dx
$$
$$
u = \ln x \implies du=\frac{1}{x}dx \implies dux=dx \implies du\cdot e^u=dx
$$
$$
I=\int \sin(u)e^udu
$$
$$
x=\sin(u) \implies dx=\cos x\cdot du, \quad dv=e^u \implies v=e^u
$$
$$
I=\sin(u)e^u - \int e^u\cos u\cdot dx
$$
$$
x=\cos(u) \implies dx=-\sin x\cdot du, \quad dv=e^u \implies v=e^u
$$
$$
I=\sin(u)e^u -\left( \cos(u)e^u - \int e^u(-\sin(x))dx \right)
$$
$$
2I= \sin(u)e^u-\cos(u)e^u
$$
$$
I= \frac{\sin(u)e^u-\cos(u)e^u}{2}
$$
 # 31
$$
 \int x \sin x
$$