# 15.
$$
I= \int\frac{1}{x(x+2)(x-1)}dx=  \int \frac{A}{x}+\frac{B}{x+2}+\frac{C}{x-1}
$$
Logo,
$$
1=A(x+2)(x-1)+B(x)(x-1)+C(x+2)(x)
$$
```python
=> x = 0
	=> 1 = A(2)(-1) + 0 + 0 <=> A = -1/2
=> x = 1
	=> 1 = 0 + 0 + C * 3 <=> C = 1/3
=> x = -2
	=> 1 = 0 + B * -6 + 0 <=> B = 1/6
```

Assim
$$
I = -\frac{1}{2}\int \frac{1}{x}dx + \frac{1}{6}\int \frac{1}{x+2}dx + \frac{1}{3} \int \frac{1}{x-1}dx
$$
$$
I = -\frac{1}{2}\ln|x|+\frac{1}{6}\ln|x+2|+\frac{1}{3}\ln|x-1|
$$

# 17.
$$
I= \int_{0}^{1} \frac{x^3}{x^2+2x+1}dx
$$
Note que:
$$
\frac{x^3}{x^2+2x+1}= x-2+ \frac{3x+2}{(x+1)^2}
$$
Assim,
$$
I=\int x -2\hspace{1mm}dx + \int w
$$
$$
w= \frac{3x+2}{(x+1)^2}= \frac{A}{(x+1)}+\frac{B}{(x+1)^2}
$$
```python
3x + 2 = A(x+1)+B

=> x = -1
	=> -1 = B <=> B = -1
=> x = 0
	=> 3x + 2 = A + B <=> A = 3

Logo,
A = 3, B = -1
```

$$
\begin{array}{l}
I = \frac{x^2}{2}-2x+3\int \frac{1}{x+1}-\int \frac{1}{(x+1)^2}\\
= \frac{x^2}{2}-2x+3\ln|x+1|+\frac{1}{x+1}\\
=\left[ \frac{x^2}{2}-2x+3\ln|x+1|+\frac{1}{x+1} \right]_{0}^{1}\\
=\left[ \frac{1}{2}-2+3\ln|2|+\frac{1}{2} \right]-[0-0+0+1] \\
=3\ln(2)-2
\end{array}
$$
# 19
$$
\begin{array}{l}
I=\int \frac{1}{(x^2-1)^2}dx \\
= \int \frac{1}{(x+1)^2(x-1)^2}dx =\int \frac{A}{(x+1)}+\frac{B}{(x+1)^2}+\frac{C}{(x-1)}+\frac{D}{(x-1)^2}\\ \\

\text{Logo,} \\ \\

1=A(x+1)(x-1)^2+B(x-1)^2+C(x-1)(x+1)^2+D(x+1)^2 \\ \\

\implies x=1 \\
\hspace{10mm} \implies 1 = 0+0+0+ D \cdot 4 \implies D = \frac{1}{4} \\
\implies x = -1 \\
\hspace{10mm} \implies 1= 0+B\cdot 4 + 0 + 0 \implies B= \frac{1}{4}\\
\implies x=0 \\
\hspace{10mm} \implies 1 = A+\frac{1}{4}-C+\frac{1}{4} \implies C = A+\frac{2}{4} \\
\implies x=2 \\
\hspace{10mm} \implies 1 = A\cdot 3+1+C\cdot 9+ \frac{9}{4} \implies 1= A \cdot 3+1+\left( A+ \frac{2}{4} \right)9+\frac{9}{4} \\
\hspace{10mm}\implies A = -\frac{1}{4} \\
\implies C = \frac{11}{4}
\end{array}
$$

